@prefix aorc: <https://github.com/Dewberry/blobfish/blob/aorc_refactor/semantics/rdf/mapped_aorc.ttl#> .
@prefix owl: <http://www.w3.org/2002/07/owl#> .
@prefix rdf: <http://www.w3.org/1999/02/22-rdf-syntax-ns#> .
@prefix rdfs: <http://www.w3.org/2000/01/rdf-schema#> .
@prefix xsd: <http://www.w3.org/2001/XMLSchema#> .

aorc:CompositeDataset a rdfs:Class,
        owl:Class ;
    rdfs:comment "A CONUS netCDF dataset created by stitching together AORC data from all RFC offices for a single hour"^^xsd:string ;
    rdfs:subClassOf <http://www.w3.org/ns/dcat#Dataset> .

aorc:CompositeDistribution a rdfs:Class,
        owl:Class ;
    rdfs:comment "The access point for the .zarr directory containing the composite dataset of all RFC office data for an hour"^^xsd:string ;
    rdfs:subClassOf <http://www.w3.org/ns/dcat#Distribution> .

aorc:CompositeJob a rdfs:Class,
        owl:Class ;
    rdfs:comment "The execution of the composite script on the docker image instance which generated the composite dataset(s)"^^xsd:string ;
    rdfs:subClassOf <http://www.w3.org/ns/prov#Activity> .

aorc:CompositeScript a rdfs:Class,
        owl:Class ;
    rdfs:comment "A script contained within the docker image which was executed in order to composite AORC dataset(s)"^^xsd:string ;
    rdfs:subClassOf <http://purl.org/dc/dcmitype/Software> .

aorc:DockerImage a rdfs:Class,
        owl:Class ;
    rdfs:comment "A docker image hosted on a repository that can be used to generate mirror datasets"^^xsd:string ;
    rdfs:subClassOf <http://purl.org/dc/dcmitype/Software> .

aorc:MirrorDataset a rdfs:Class,
        owl:Class ;
    rdfs:comment "An AORC dataset that has been copied from its original location on NOAA servers to s3"^^xsd:string ;
    rdfs:subClassOf <http://www.w3.org/ns/dcat#Dataset> .

aorc:MirrorDistribution a rdfs:Class,
        owl:Class ;
    rdfs:comment "The access point for the mirrored dataset on s3"^^xsd:string ;
    rdfs:subClassOf <http://www.w3.org/ns/dcat#Distribution> .

aorc:PrecipPartition a rdfs:Class,
        owl:Class ;
    rdfs:comment "The directory which directly holds all source datasets which are published by the creator RFC office associated with the PrecipPartition"^^xsd:string ;
    rdfs:subClassOf <http://www.w3.org/ns/dcat#Catalog> .

aorc:RFC a rdfs:Class,
        owl:Class ;
    rdfs:comment "The River Forecast Center which is associated with the coverage area for a catalog of precipitation data"^^xsd:string ;
    rdfs:subClassOf <http://xmlns.com/foaf/0.1/Organization> .

aorc:SourceDataset a rdfs:Class,
        owl:Class ;
    rdfs:comment "The AORC dataset in its original location on the NOAA servers"^^xsd:string ;
    rdfs:subClassOf <http://www.w3.org/ns/dcat#Dataset> .

aorc:SourceDistribution a rdfs:Class,
        owl:Class ;
    rdfs:comment "The access point for the mirrored dataset on s3"^^xsd:string ;
    rdfs:subClassOf <http://www.w3.org/ns/dcat#Distribution> .

aorc:TransferJob a rdfs:Class,
        owl:Class ;
    rdfs:comment "The execution of the transfer script on the docker image instance which generated the mirror dataset(s)"^^xsd:string ;
    rdfs:subClassOf <http://www.w3.org/ns/prov#Activity> .

aorc:TransferScript a rdfs:Class,
        owl:Class ;
    rdfs:comment "A script contained within the docker image which was executed in order to mirror the dataset(s)"^^xsd:string ;
    rdfs:subClassOf <http://purl.org/dc/dcmitype/Software> .

aorc: a owl:Ontology .

aorc:hasCompositeDataset a rdf:Property,
        owl:ObjectProperty ;
    rdfs:comment "Indicates that the subject dataset was used in the creation of the object composite dataset"^^xsd:string ;
    rdfs:domain <http://www.w3.org/ns/dcat#Dataset> ;
    rdfs:range aorc:CompositeDataset ;
    owl:inverseOf aorc:isCompositeOf .

aorc:hasMirrorDataset a rdf:Property,
        owl:ObjectProperty ;
    rdfs:comment "Indicates what mirror dataset the subject source dataset was used to generate"^^xsd:string ;
    owl:inverseOf aorc:hasSourceDataset .

aorc:hasRFCAlias a owl:DatatypeProperty ;
    rdfs:comment "The 2 character alias assigned to an RFC office (ex: 'LM' for Lower Mississippi River Forecast Office)"^^xsd:string ;
    owl:equivalentProperty <http://purl.org/dc/terms/alternative> .

aorc:hasRFCName a owl:DatatypeProperty ;
    rdfs:comment "The full region name for the RFC office (ex: 'LOWER MISSISSIPPI for Lower Mississippi River Forecast Center)"^^xsd:string ;
    owl:equivalentProperty <http://purl.org/dc/terms/title> .

aorc:isCompositeScriptOf a rdf:Property,
        owl:ObjectProperty ;
    rdfs:comment "Indicates to what software the script belongs"^^xsd:string ;
    rdfs:subPropertyOf <http://purl.org/dc/terms/isPartOf> ;
    owl:inverseOf aorc:hasCompositeScript .

aorc:isDockerImageOf a rdf:Property,
        owl:ObjectProperty ;
    rdfs:comment "Indicates what software belong to the docker image"^^xsd:string ;
    rdfs:subPropertyOf <http://purl.org/dc/terms/hasPart> ;
    owl:inverseOf aorc:hasDockerImage .

aorc:isMirrorDatasetOf a rdf:Property,
        owl:ObjectProperty ;
    rdfs:comment "Indicates the origin of the subject mirrored dataset"^^xsd:string ;
    rdfs:domain aorc:MirrorDataset ;
    rdfs:range aorc:SourceDataset ;
    rdfs:subPropertyOf <http://purl.org/dc/terms/source> .

aorc:isRFCOf a rdf:Property,
        owl:ObjectProperty ;
    rdfs:comment "Indicates the data resources that have been published by the subject RFC Office"^^xsd:string ;
    owl:inverseOf aorc:hasRFC .

aorc:isSourceDatasetOf a rdf:Property,
        owl:ObjectProperty ;
    rdfs:comment "Indicates what mirror dataset the subject source dataset was used to generate"^^xsd:string ;
    owl:inverseOf aorc:hasSourceDataset .

aorc:isTransferScriptOf a rdf:Property,
        owl:ObjectProperty ;
    rdfs:comment "Indicates to what software the script belongs"^^xsd:string ;
    rdfs:subPropertyOf <http://purl.org/dc/terms/isPartOf> ;
    owl:inverseOf aorc:hasTransferScript .

aorc:wasCompositedBy a rdf:Property,
        owl:ObjectProperty ;
    rdfs:comment "Indicates the job that was responsible for creating the subject composite dataset"^^xsd:string ;
    rdfs:subPropertyOf <http://www.w3.org/ns/prov#wasGeneratedBy> ;
    owl:inverseOf aorc:createdComposite .

aorc:wasTransferredBy a rdf:Property,
        owl:ObjectProperty ;
    rdfs:comment "Indicates the job that was responsible for transferring the subject mirror dataset"^^xsd:string ;
    rdfs:subPropertyOf <http://www.w3.org/ns/prov#wasGeneratedBy> ;
    owl:inverseOf aorc:transferred .

aorc:createdComposite a rdf:Property,
        owl:ObjectProperty ;
    rdfs:comment "Indicates the job that was responsible for the creation of the subject composite image"^^xsd:string ;
    rdfs:domain aorc:CompositeJob ;
    rdfs:range aorc:CompositeDataset ;
    rdfs:subPropertyOf <http://www.w3.org/ns/prov#generated> .

aorc:hasCompositeScript a rdf:Property,
        owl:ObjectProperty ;
    rdfs:comment "Indicates what scripts belong to the software"^^xsd:string ;
    rdfs:domain <http://purl.org/dc/dcmitype/Software> ;
    rdfs:range aorc:CompositeScript ;
    rdfs:subPropertyOf <http://purl.org/dc/terms/hasPart> .

aorc:hasDockerImage a rdf:Property,
        owl:ObjectProperty ;
    rdfs:comment "Indicates what docker image to which the software belongs"^^xsd:string ;
    rdfs:domain <http://purl.org/dc/dcmitype/Software> ;
    rdfs:range aorc:DockerImage ;
    rdfs:subPropertyOf <http://purl.org/dc/terms/isPartOf> .

aorc:hasRFC a rdf:Property,
        owl:ObjectProperty ;
    rdfs:comment "Indicates the RFC Office responsible for the publication of the subject data resource"^^xsd:string ;
    rdfs:domain <http://www.w3.org/ns/dcat#Resource> ;
    rdfs:range aorc:RFC ;
    rdfs:subPropertyOf <http://purl.org/dc/terms/creator> .

aorc:hasTransferScript a rdf:Property,
        owl:ObjectProperty ;
    rdfs:comment "Indicates what scripts belong to the software"^^xsd:string ;
    rdfs:domain <http://purl.org/dc/dcmitype/Software> ;
    rdfs:range aorc:TransferScript ;
    rdfs:subPropertyOf <http://purl.org/dc/terms/hasPart> .

aorc:isCompositeOf a rdf:Property,
        owl:ObjectProperty ;
    rdfs:comment "Indicates what datasets were combined to create the subject composite dataset"^^xsd:string ;
    rdfs:domain aorc:CompositeDataset ;
    rdfs:range <http://www.w3.org/ns/dcat#Dataset> ;
    rdfs:subPropertyOf <http://purl.org/dc/terms/source> .

aorc:transferred a rdf:Property,
        owl:ObjectProperty ;
    rdfs:comment "Indicates the mirror dataset that the subject job transferred"^^xsd:string ;
    rdfs:domain aorc:TransferJob ;
    rdfs:range aorc:MirrorDataset ;
    rdfs:subPropertyOf <http://www.w3.org/ns/prov#generated> .

aorc:hasSourceDataset a rdf:Property,
        owl:ObjectProperty ;
    rdfs:comment "Indicates the origin of the subject mirrored dataset"^^xsd:string ;
    rdfs:domain aorc:MirrorDataset ;
    rdfs:range aorc:SourceDataset ;
    rdfs:subPropertyOf <http://purl.org/dc/terms/source> .

[] a owl:AllDisjointClasses ;
    owl:members ( aorc:CompositeDataset aorc:CompositeDistribution aorc:CompositeScript aorc:CompositeJob aorc:DockerImage aorc:MirrorDataset aorc:MirrorDistribution aorc:PrecipPartition aorc:RFC aorc:SourceDataset aorc:SourceDistribution aorc:TransferJob aorc:TransferScript ) .

